test/snapshots/Test_union_nested_owns_with_functional_spec_maybe_freeable.fst
@@ -1,0 +1,297 @@
+module Test_union_nested_owns_with_functional_spec_maybe_freeable
+
+#lang-pulse
+#set-options "--ext pulse:no_admit_diag"
+
+open Pulse
+open Pulse.Lib.C
+
+
+
+module U32 = Pulse.Lib.C.UInt32 open Pulse.Lib.C.UInt32
+noeq
+type ab = {
+a: ref (ref UInt32.t);
+b: ref (ref bool);
+}
+
+noeq
+type ab_spec = 
+ | Case_ab_a of (ref UInt32.t)
+ | Case_ab_b of (ref bool)
+
+let ab_pred(u : ref ab) (s : ab_spec) : slprop =
+exists* uv. (u |-> uv) **
+begin match s with
+ | Case_ab_a v -> uv.a |-> v
+ | Case_ab_b v -> uv.b |-> v
+end
+
+ghost fn ab_explode (x : ref ab) (#s : ab_spec)
+requires ab_pred x s
+ensures exists* (v : ab). (x |-> v) **
+begin match s with
+ | Case_ab_a w -> v.a |-> w
+ | Case_ab_b w -> v.b |-> w
+end
+{
+unfold ab_pred;
+}
+
+ghost
+fn ab_recover (x : ref ab) (#s : ab_spec)
+requires exists* (v : ab). (x |-> v) **
+begin match s with
+ | Case_ab_a w -> v.a|-> w
+ | Case_ab_b w -> v.b|-> w
+end
+ensures ab_pred x s
+{
+fold (ab_pred x s);
+}
+
+ghost
+fn ab_change_a(x : ref ab)
+requires exists* s. ab_pred x s
+ensures exists* s. ab_pred x (Case_ab_a s)
+{ admit() }
+
+ghost
+fn ab_change_b(x : ref ab)
+requires exists* s. ab_pred x s
+ensures exists* s. ab_pred x (Case_ab_b s)
+{ admit() }
+
+ghost
+fn ab_is_a(x : ref ab) (#s:_{Case_ab_a? s})
+requires ab_pred x s
+ensures  ab_pred x (Case_ab_a(Case_ab_a?._0 s))
+{ admit() }
+
+ghost
+fn ab_is_b(x : ref ab) (#s:_{Case_ab_b? s})
+requires ab_pred x s
+ensures  ab_pred x (Case_ab_b(Case_ab_b?._0 s))
+{ admit() }
+
+fn incr_a
+(x : ( ref ab) )
+(#a:erased (ref uint32))
+(#v:erased uint32)
+preserves ab_pred x (Case_ab_a a)
+requires reveal a |-> v
+requires pure (U32.fits ( + ) (UInt32.v v) 1)
+ensures exists* (u:uint32). (reveal a |-> u) ** pure (U32.as_int u == U32.as_int v + 1)
+{
+let mut x : (ref ab) = x;
+ab_is_a (!x);
+ab_explode !x;
+(! (! (! x)).a) := (UInt32.add (! (! (! (! x)).a)) (int32_to_uint32 1l));
+ab_recover !x #(Case_ab_a _);
+}
+
+fn set_case_a
+(x : ( ref ab) )
+(a : ( ref UInt32.t) )
+(#v:erased _)
+requires exists* s. ab_pred x s
+preserves a |-> v
+ensures ab_pred x (Case_ab_a a)
+{
+let mut x : (ref ab) = x;
+let mut a : (ref UInt32.t) = a;
+ab_change_a !x;
+ab_explode !x;
+Mkab?.a (! (! x)) := (! a);
+ab_recover !x #(Case_ab_a _);
+}
+
+noeq
+type stru = {
+tag: ref Int8.t;
+payload: ref ab;
+}
+
+[@@erasable]
+noeq
+type stru_spec = {
+tag : Int8.t;
+payload : ab_spec
+
+}
+
+[@@pulse_unfold]
+let stru_pred ([@@@mkey]x:ref stru) (s:stru_spec) : slprop =
+exists* (y: stru). (x |-> y) **
+(y.tag |-> s.tag) **
+ab_pred y.payload s.payload
+
+assume val stru_spec_default : stru_spec
+
+assume val stru_default (stru_var_spec:stru_spec) : stru
+
+ghost
+fn stru_pack (stru_var:ref stru) (#stru_var_spec:stru_spec)
+requires stru_var|-> stru_default stru_var_spec
+ensures exists* v. stru_pred stru_var v ** pure (v == stru_var_spec)
+{ admit() }
+
+ghost
+fn stru_unpack (stru_var:ref stru)
+requires exists* v. stru_pred stru_var v 
+ensures exists* u. stru_var |-> u
+{ admit() }
+
+fn stru_alloc ()
+returns x:ref stru
+ensures freeable x
+ensures exists* v. stru_pred x v
+{ admit () }
+
+fn stru_free (x:ref stru)
+requires freeable x
+requires exists* v. stru_pred x v
+{ admit() }
+
+
+ghost fn stru_explode (x:ref stru) (#s:stru_spec)
+requires stru_pred x s
+ensures exists* (v: stru). (x |-> v) ** (v.tag |-> s.tag) ** 
+(v.payload `ab_pred` s.payload)
+
+{unfold stru_pred}
+
+
+ghost
+fn stru_recover (x:ref stru) (#a0 : Int8.t)
+(#a1 : ab_spec)
+
+requires exists* (y: stru). (x |-> y) ** 
+(y.tag |-> a0) **
+(y.payload  `ab_pred` a1)
+ensures exists* w. stru_pred x w ** pure (w == {tag = a0;
+payload = a1})
+{fold stru_pred x ({tag = a0;
+payload = a1}) }
+
+let maybe_freeable #a (b:_Bool) (r:ref a) = if b then freeable r else emp let stru_payload (a: ab_spec) (s: either uint32 _Bool) (free:_Bool) : slprop = match a with | Case_ab_a a -> exists* v. (a |-> v) ** maybe_freeable free a ** pure (s == Inl v) | Case_ab_b b -> exists* v. (b |-> v) ** maybe_freeable free b ** pure (s == Inr v) [@@ pulse_unfold] let tag_relation (s:stru_spec): slprop = pure (match s.tag with | 0y -> Case_ab_a? s.payload | 1y -> Case_ab_b? s.payload | _ -> False) [@@ pulse_unfold] let stru_ok_aux (u: ref stru) (ib: either uint32 _Bool) (f:_Bool) (s:_) : slprop = stru_pred u s ** stru_payload s.payload ib f ** tag_relation s [@@ pulse_unfold] let stru_ok (u: ref stru) (ib: either uint32 _Bool) (f:_Bool) : slprop = exists* s. stru_ok_aux u ib f s ghost fn elim_stru_payload_a (a:ab_spec { Case_ab_a? a }) (#ib #f:_) requires stru_payload a ib f ensures exists* v. (Case_ab_a?._0 a |-> v) ** (maybe_freeable f (Case_ab_a?._0 a)) ** pure (ib == Inl v) { rewrite each a as (Case_ab_a (Case_ab_a?._0 a)); unfold stru_payload; } ghost fn elim_stru_payload_b (a:ab_spec { Case_ab_b? a }) (#ib #f:_) requires stru_payload a ib f ensures exists* v. (Case_ab_b?._0 a |-> v) ** (maybe_freeable f (Case_ab_b?._0 a)) ** pure (ib == Inr v) { rewrite each a as (Case_ab_b (Case_ab_b?._0 a)); unfold stru_payload; } ghost fn intro_stru_payload_a (a:ab_spec { Case_ab_a? a }) (#f:_Bool) (#v:_) requires (Case_ab_a?._0 a |-> v) ** maybe_freeable f (Case_ab_a?._0 a) ensures stru_payload (Case_ab_a (Case_ab_a?._0 a)) (Inl v) f { fold stru_payload (Case_ab_a (Case_ab_a?._0 a)) (Inl v) f } ghost fn intro_stru_payload_b (a:ab_spec { Case_ab_b? a }) (#v:_) #f requires (Case_ab_b?._0 a |-> v) ** maybe_freeable f (Case_ab_b?._0 a) ensures stru_payload (Case_ab_b (Case_ab_b?._0 a)) (Inr v) f { fold stru_payload (Case_ab_b (Case_ab_b?._0 a)) (Inr v) f } ghost fn intro_stru_ok (u:ref stru) (#s:stru_spec) (#pl:ab_spec) (#ib:_) #f requires stru_pred u s ** stru_payload pl ib f ** pure (s.payload == pl) ** pure (match s.tag with | 0y -> Case_ab_a? s.payload | 1y -> Case_ab_b? s.payload | _ -> False ) ensures stru_ok u ib f { rewrite each pl as s.payload; } ghost fn tag_relation_lemma (y:ref stru) (#ib: either uint32 _Bool) #f (#s:stru_spec) preserves stru_ok_aux y ib f s ensures pure (Inl? ib <==> s.tag==0y) ensures pure (Inr? ib <==> s.tag==1y) { let v = s.tag; if (v = 0y) { ab_is_a _; elim_stru_payload_a _; intro_stru_payload_a _; } else if (v = 1y) { ab_is_b _; elim_stru_payload_b _; intro_stru_payload_b _; } else { unreachable() } }
+fn test_union
+(foo : ( ref stru) )
+(#s:erased (either uint32 _Bool))
+(#f:erased _Bool)
+requires stru_ok foo s f
+ensures exists* (t:either uint32 _Bool). stru_ok foo t f ** pure (match s with | Inl _ -> t == Inl 1ul | Inr _ -> Inr? t && not (Inr?.v t))
+{
+let mut foo : (ref stru) = foo;
+stru_explode (!foo);
+if((int32_to_bool (bool_to_int32 (Int32.eq (int8_to_int32 (! (! (! foo)).tag)) 0l))))
+{
+ab_is_a (! (! foo)).payload; ab_explode (! (!foo)).payload; elim_stru_payload_a _;
+(! (! (! (! foo)).payload).a) := (int32_to_uint32 1l);
+intro_stru_payload_a _; ab_recover (! (!foo)).payload #(Case_ab_a _); stru_recover (!foo); intro_stru_ok (!foo);
+}
+else
+{
+if((int32_to_bool (bool_to_int32 (Int32.eq (int8_to_int32 (! (! (! foo)).tag)) 1l))))
+{
+ab_is_b (! (! foo)).payload; ab_explode (! (!foo)).payload; elim_stru_payload_b _;
+(! (! (! (! foo)).payload).b) := (int32_to_bool 0l);
+intro_stru_payload_b _; ab_recover (! (!foo)).payload #(Case_ab_b _); stru_recover (!foo); intro_stru_ok (!foo);
+}
+else
+{
+unreachable();
+};
+};
+}
+
+fn test_union_a
+(foo : ( ref stru) )
+(#s:erased (either uint32 _Bool) { Inl? s })
+(#f:erased _Bool)
+requires stru_ok foo s f
+ensures stru_ok foo (Inl 1ul) f
+{
+let mut foo : (ref stru) = foo;
+tag_relation_lemma _; stru_explode (!foo);
+ab_is_a (! (! foo)).payload; ab_explode (! (!foo)).payload; elim_stru_payload_a _;
+(! (! (! (! foo)).payload).a) := (int32_to_uint32 1l);
+intro_stru_payload_a _; ab_recover (! (!foo)).payload #(Case_ab_a _); stru_recover (!foo); intro_stru_ok (!foo);
+}
+
+fn test_union_a_alt
+(foo : ( ref stru) )
+(#s:erased uint32)
+(#f:erased _Bool)
+requires stru_ok foo (Inl #uint32 s) f
+ensures stru_ok foo (Inl 1ul) f
+{
+let mut foo : (ref stru) = foo;
+tag_relation_lemma _; stru_explode (!foo);
+ab_is_a (! (! foo)).payload; ab_explode (! (!foo)).payload; elim_stru_payload_a _;
+(! (! (! (! foo)).payload).a) := (int32_to_uint32 1l);
+intro_stru_payload_a _; ab_recover (! (!foo)).payload #(Case_ab_a _); stru_recover (!foo); intro_stru_ok (!foo);
+}
+
+fn test_union_a_alt2
+(foo : ( ref stru) )
+(#s:erased uint32)
+(#f:erased _Bool)
+requires stru_ok foo (Inl #uint32 s) f
+ensures exists* v. stru_ok foo v f ** pure (v == Inl 1ul)
+{
+let mut foo : (ref stru) = foo;
+tag_relation_lemma _; stru_explode (!foo);
+ab_is_a (! (! foo)).payload; ab_explode (! (!foo)).payload; elim_stru_payload_a _;
+(! (! (! (! foo)).payload).a) := (int32_to_uint32 1l);
+intro_stru_payload_a _; ab_recover (! (!foo)).payload #(Case_ab_a _); stru_recover (!foo); intro_stru_ok (!foo);
+}
+
+[@@expect_failure [17]]
+fn test_union_b_alt
+(foo : ( ref stru) )
+(#s:erased _Bool)
+(#f:erased _Bool)
+requires stru_ok foo (Inr #_ #_Bool s) f
+ensures stru_ok foo (Inr (not s)) f
+{
+let mut foo : (ref stru) = foo;
+tag_relation_lemma _; stru_explode (!foo);
+ab_is_b (! (! foo)).payload; ab_explode (! (!foo)).payload; elim_stru_payload_b _;
+(! (! (! (! foo)).payload).b) := (int32_to_bool (bool_to_int32 (not (! ((! (! (! (! foo)).payload).b))))));
+intro_stru_payload_b _; ab_recover (! (!foo)).payload #(Case_ab_b _); stru_recover (!foo); intro_stru_ok (!foo);
+}
+
+fn test_union_b_alt2
+(foo : ( ref stru) )
+(#s:erased _Bool)
+(#f:erased _Bool)
+requires stru_ok foo (Inr #_ #_Bool s) f
+ensures exists* v. stru_ok foo v f ** pure (v == Inr (not s))
+{
+let mut foo : (ref stru) = foo;
+tag_relation_lemma _; stru_explode (!foo);
+ab_is_b (! (! foo)).payload; ab_explode (! (!foo)).payload; elim_stru_payload_b _;
+(! (! (! (! foo)).payload).b) := (int32_to_bool (bool_to_int32 (not (! ((! (! (! (! foo)).payload).b))))));
+intro_stru_payload_b _; ab_recover (! (!foo)).payload #(Case_ab_b _); stru_recover (!foo); intro_stru_ok (!foo);
+}
+
+[@pulse_unfold] let ab_cases (uv:ab) (s:ab_spec) : slprop = begin match s with | Case_ab_a v -> uv.a |-> v | Case_ab_b v -> uv.b |-> v end assume val ab_spec_default : ab_spec assume val ab_default (ab_var_spec:ab_spec) : ab instance ab_inhabited : inhabited ab = { witness = (ab_default ab_spec_default) } ghost fn ab_pack (ab_var:ref ab) (#ab_spec:ab_spec) requires ab_var|-> ab_default ab_spec ensures exists* v. ab_pred ab_var v ** pure (v == ab_spec) { admit() } ghost fn ab_unpack (ab_var:ref ab) (#v:ab_spec) requires ab_pred ab_var v ensures exists* ab. (ab_var |-> ab) ** ab_cases ab v { admit() } ghost fn ab_explode_drop (x : ref ab) (#s : ab_spec) requires ab_pred x s ensures exists* (v : ab). (x |-> v) { ab_explode x; drop_ (match s with | Case_ab_a _ -> _ | Case_ab_b _ -> _); } ghost fn intro_maybe_freeable a (r:ref a) requires freeable r ensures maybe_freeable _true_ r { fold (maybe_freeable _true_ r) }
+fn mk_union_a ()
+returns x:ref stru
+ensures exists* v. stru_ok x v _true_ ** pure (v == Inl 0ul) ** freeable x
+{
+let mut a : (ref UInt32.t) = alloc_ref #UInt32.t ();
+intro_maybe_freeable _ (!a);
+(! a) := (uint64_to_uint32 0UL);
+let mut ab: ab = witness #_ #_;
+ab_pack ab;
+(set_case_a (ab) (! a));
+let mut x : (ref stru) = stru_alloc ();
+stru_explode (!x);
+Mkstru?.tag (! (! x)) := (int32_to_int8 0l);
+ab_unpack ab; ab_explode_drop (!(!x)).payload;
+Mkstru?.payload (! (! x)) := (! ab);
+intro_stru_payload_a (Case_ab_a (!a)); ab_recover (!(!x)).payload #(Case_ab_a _); stru_recover (!x); intro_stru_ok (!x);
+(! x);
+}
